src/Common/CommonStreams.v
@@ -3,19 +3,6 @@ From Coq Require Import Streams.
 
 (** Additional streams utilities *)
 
-Section decompose.
-  Context {A : Type}.
-
-  Definition Stream_decompose (s : Stream A) : Stream A :=
-    match s with Cons a sa => Cons a sa end.
-
-  Lemma Stream_decompose_thm : forall (s : Stream A),
-      s = Stream_decompose s.
-  Proof.
-    intros s. case s; simpl; trivial.
-  Qed.
-End decompose.
-
 Section map.
   Context {A B : Type}.
 
@@ -25,7 +12,7 @@ Section map.
       (map f (Cons a sa)) = (Cons (f a) (map f sa)).
   Proof.
     intros a sa; simpl.
-    rewrite Stream_decompose_thm at 1; reflexivity.
+    rewrite unfold_Stream at 1; reflexivity.
   Qed.
 End map.
 
@@ -44,7 +31,7 @@ Section map2.
       (map2 (Cons a sa) (Cons b sb)) = (Cons (f a b) (map2 sa sb)).
   Proof.
     intros a b sa sb; simpl.
-    rewrite Stream_decompose_thm at 1; reflexivity.
+    rewrite unfold_Stream at 1; reflexivity.
   Qed.
 
   Lemma map2_hd : forall (sa : Stream A) (sb : Stream B),
