src/Lustre/Normalization/Idempotence.v
@@ -1,0 +1,345 @@
+From Coq Require Import List Sorting.Permutation.
+Import List.ListNotations.
+Open Scope list_scope.
+Require Import Omega.
+Require Import ProofIrrelevance.
+
+From Velus Require Import Common Ident.
+From Velus Require Import Operators.
+From Velus Require Import Lustre.LSyntax Lustre.LOrdered Lustre.LTyping.
+From Velus Require Import Lustre.Normalization.Fresh Lustre.Normalization.FullNorm.
+
+(** * Idempotence of the normalization *)
+
+Local Set Warnings "-masking-absolute-name".
+Module Type IDEMPOTENCE
+       (Import Ids : IDS)
+       (Import Op : OPERATORS)
+       (OpAux : OPERATORS_AUX Op)
+       (Import Syn : LSYNTAX Ids Op)
+       (Import Norm : FULLNORM Ids Op OpAux Syn).
+
+  Import Fresh Fresh.Fresh Facts Tactics.
+
+  (** ** Idempotence of normalization *)
+
+  Fact normalized_lexp_normalize_idem : forall e is_control st,
+      normalized_lexp e ->
+      normalize_exp is_control e st = ([e], [], st).
+  Proof with eauto.
+    intros e is_control st Hnormed; revert is_control.
+    induction Hnormed; intro is_control; simpl; repeat inv_bind...
+    - (* unop *)
+      repeat eexists...
+      inv_bind...
+    - (* binop *)
+      repeat eexists...
+      inv_bind. repeat eexists...
+      inv_bind...
+    - (* when *)
+      exists [e]. exists []. exists st.
+      repeat split; inv_bind...
+      exists [[e]]. exists [[]]. exists st.
+      repeat split; simpl; inv_bind...
+      repeat eexists...
+      inv_bind.
+      repeat eexists; inv_bind...
+  Qed.
+
+  Corollary normalized_lexps_normalize_idem' : forall es is_control st,
+      Forall normalized_lexp es ->
+      (exists eqs, map_bind2 (normalize_exp is_control) es st = (List.map (fun e => [e]) es, eqs, st) /\ (concat eqs = [])).
+  Proof with eauto.
+    induction es; intros is_control st Hf;
+      inv Hf; simpl; repeat inv_bind...
+    eapply normalized_lexp_normalize_idem in H1...
+    eapply (IHes is_control st) in H2; clear IHes.
+    destruct H2 as [eqs [H2 Heqs]].
+    exists ([]::eqs).
+    repeat eexists... inv_bind.
+    repeat eexists... inv_bind.
+    repeat eexists... inv_bind.
+    repeat f_equal.
+  Qed.
+
+  Corollary normalized_lexps_normalize_idem : forall es st,
+      Forall normalized_lexp es ->
+      normalize_exps es st = (es, [], st).
+  Proof with eauto.
+    intros.
+    eapply normalized_lexps_normalize_idem' in H. destruct H as [eqs [H Heqs]].
+    unfold normalize_exps; inv_bind.
+    repeat eexists...
+    inv_bind. rewrite concat_map_singl1. congruence.
+  Qed.
+
+  Fact normalized_cexp_normalize_idem : forall e st,
+      normalized_cexp e ->
+      normalize_exp true e st = ([e], [], st).
+  Proof with eauto.
+    intros e st Hnormed.
+    induction Hnormed; simpl; repeat inv_bind...
+    - (* merge *)
+      exists [et]. exists []. exists st.
+      repeat split; inv_bind...
+      + exists [[et]]. exists [[]]. exists st.
+        repeat split; simpl; inv_bind...
+        repeat eexists...
+        inv_bind.
+        repeat eexists; inv_bind...
+      + exists [ef]. exists []. exists st.
+        repeat split; simpl; inv_bind...
+        exists [[ef]]. exists [[]]. exists st.
+        repeat split; simpl; inv_bind...
+        repeat eexists...
+        inv_bind.
+        repeat eexists; inv_bind...
+    - (* ite *)
+      eapply normalized_lexp_normalize_idem in H. repeat eexists...
+      repeat inv_bind.
+      exists [et]. exists []. exists st.
+      repeat split; inv_bind...
+      + exists [[et]]. exists [[]]. exists st.
+        repeat split; simpl; inv_bind...
+        repeat eexists...
+        inv_bind.
+        repeat eexists; inv_bind...
+      + exists [ef]. exists []. exists st.
+        repeat split; simpl; inv_bind...
+        exists [[ef]]. exists [[]]. exists st.
+        repeat split; simpl; inv_bind...
+        repeat eexists...
+        inv_bind.
+        repeat eexists; inv_bind...
+    - (* lexp *) eapply normalized_lexp_normalize_idem...
+  Qed.
+
+  Fact normalize_fby_idem : forall e0 e ann st,
+      is_constant e0 ->
+      normalized_lexp e ->
+      normalize_fby [e0] [e] [ann] st = ([Efby [e0] [e] [ann]], [], st).
+  Proof with eauto.
+    intros e0 e [ty cl] st Hcons Hnormed.
+    unfold normalize_fby; inv_bind.
+    eexists. exists [[]]. exists st. split; simpl; inv_bind...
+    eexists. exists []. exists st. split; simpl.
+    - unfold fby_iteexp.
+      destruct (Norm.is_constant e0) eqn:Hisconstant; repeat inv_bind...
+      rewrite <- is_constant_is_constant in Hcons. congruence.
+    - inv_bind.
+      repeat eexists; inv_bind...
+  Qed.
+
+  Fact normalized_rhs_normalize_idem : forall e keep_fby st,
+      normalized_rhs keep_fby e ->
+      normalize_rhs keep_fby e st = ([e], [], st).
+  Proof with eauto.
+    intros e keep_fby st Hnormed.
+    destruct e; inv Hnormed; unfold normalize_rhs;
+      try (solve [eapply normalized_cexp_normalize_idem; eauto]);
+      try (solve [inv H; inv H0]).
+    - (* fby *)
+      repeat inv_bind.
+      exists [e0]. exists []. exists st.
+      split; unfold normalize_exps; inv_bind.
+      + exists [[e0]]. exists [[]]. exists st. split; simpl; inv_bind...
+        eapply constant_normalized_lexp in H2. eapply normalized_lexp_normalize_idem in H2.
+        repeat eexists...
+        inv_bind.
+        exists []. exists []. exists st.
+        repeat split; inv_bind...
+      + exists [e]. exists []. exists st. split; simpl; inv_bind...
+        * exists [[e]]. exists [[]]. exists st. split; simpl; inv_bind...
+          eapply normalized_lexp_normalize_idem in H4.
+          repeat eexists... inv_bind.
+          repeat eexists; inv_bind...
+        * repeat eexists; try inv_bind...
+          eapply normalize_fby_idem...
+    - (* app *)
+      repeat inv_bind.
+      eapply normalized_lexps_normalize_idem in H1.
+      repeat eexists... repeat inv_bind.
+      repeat eexists...
+      inv_bind...
+    - (* app (reset) *)
+      repeat inv_bind.
+      eapply normalized_lexps_normalize_idem in H1.
+      repeat (repeat eexists; eauto; simpl; inv_bind; eauto).
+  Qed.
+
+  Corollary normalized_rhss_normalize_idem' : forall es keep_fby st,
+      Forall (normalized_rhs keep_fby) es ->
+      (exists eqs, map_bind2 (normalize_rhs keep_fby) es st = (List.map (fun e => [e]) es, eqs, st) /\ (concat eqs = [])).
+  Proof with eauto.
+    induction es; intros keep_fby st Hf;
+      inv Hf; simpl; repeat inv_bind...
+    eapply normalized_rhs_normalize_idem in H1...
+    eapply (IHes keep_fby st) in H2; clear IHes.
+    destruct H2 as [eqs [H2 Heqs]].
+    exists ([]::eqs).
+    repeat (repeat eexists; eauto; inv_bind).
+  Qed.
+
+  Corollary normalized_rhss_normalize_idem : forall es keep_fby st,
+      Forall (normalized_rhs keep_fby) es ->
+      normalize_rhss keep_fby es st = (es, [], st).
+  Proof with eauto.
+    intros.
+    eapply normalized_rhss_normalize_idem' in H. destruct H as [eqs [H Heqs]].
+    unfold normalize_rhss; inv_bind.
+    repeat eexists...
+    inv_bind. rewrite concat_map_singl1. congruence.
+  Qed.
+
+  Fact normalized_equation_normalize_idem : forall G eq to_cut st,
+      wl_equation G eq ->
+      normalized_equation to_cut eq ->
+      normalize_equation to_cut eq st = ([eq], st).
+  Proof with eauto.
+    intros G [xs es] to_cut st Hwl Hnormed. inv Hwl.
+    specialize (normalized_equation_normalized_rhs _ _ _ Hnormed) as Hnormed2.
+    apply normalized_rhss_normalize_idem with (st:=st) in Hnormed2.
+    inv Hnormed; simpl; repeat inv_bind;
+      repeat eexists; eauto;
+        inv_bind; rewrite app_nil_r;
+          simpl in *; repeat f_equal.
+    - rewrite app_nil_r in H0.
+      apply firstn_all2. rewrite H0. apply le_refl.
+    - rewrite app_nil_r in H0.
+      apply firstn_all2. rewrite H0. apply le_refl.
+    - rewrite app_nil_r in H0. rewrite length_annot_numstreams in H0.
+      apply firstn_all2. simpl. rewrite H0. apply le_refl.
+  Qed.
+
+  Corollary normalized_equations_normalize_idem : forall G eqs to_cut st,
+      Forall (wl_equation G) eqs ->
+      Forall (normalized_equation to_cut) eqs ->
+      normalize_equations to_cut eqs st = (eqs, st).
+  Proof with eauto.
+    induction eqs; intros to_cut st Hwl Hnormed; inv Hwl; inv Hnormed;
+      unfold normalize_equations; repeat inv_bind...
+    eapply normalized_equation_normalize_idem in H3...
+    repeat eexists... inv_bind.
+    repeat eexists... inv_bind.
+    rewrite <- cons_is_app...
+  Qed.
+
+  Definition transport1 {n1 n2 : node} (Hin : n_in n1 = n_in n2) : 0 < length (n_in n1) -> 0 < length (n_in n2).
+  Proof. intros. induction Hin. auto. Defined.
+
+  Definition transport2 {n1 n2 : node} (Hout : n_out n1 = n_out n2) : 0 < length (n_out n1) -> 0 < length (n_out n2).
+  Proof. intros. induction Hout. auto. Defined.
+
+  Definition transport3 {n1 n2 : node}
+             (Heqs : n_eqs n1 = n_eqs n2)
+             (Hvars : n_vars n1 = n_vars n2)
+             (Hout : n_out n1 = n_out n2) :
+    Permutation (vars_defined (n_eqs n1)) (map fst ((n_vars n1) ++ (n_out n1))) ->
+    Permutation (vars_defined (n_eqs n2)) (map fst ((n_vars n2) ++ (n_out n2))).
+  Proof.
+    intros.
+    induction Heqs. induction Hvars. induction Hout.
+    auto.
+  Defined.
+
+  Definition transport4 {n1 n2 : node}
+             (Hin : n_in n1 = n_in n2)
+             (Hvars : n_vars n1 = n_vars n2)
+             (Hout : n_out n1 = n_out n2)
+             (Heqs : n_eqs n1 = n_eqs n2):
+    NoDupMembers (n_in n1 ++ n_vars n1 ++ n_out n1 ++ anon_in_eqs (n_eqs n1)) ->
+    NoDupMembers (n_in n2 ++ n_vars n2 ++ n_out n2 ++ anon_in_eqs (n_eqs n2)).
+  Proof.
+    intros.
+    induction Hin. induction Hvars. induction Hout. induction Heqs.
+    auto.
+  Defined.
+
+  Definition transport5 {n1 n2 : node}
+             (Hname : n_name n1 = n_name n2)
+             (Hin : n_in n1 = n_in n2)
+             (Hvars : n_vars n1 = n_vars n2)
+             (Hout : n_out n1 = n_out n2) :
+    Forall ValidId (n_in n1 ++ n_vars n1 ++ n_out n1) /\ valid (n_name n1) ->
+    Forall ValidId (n_in n2 ++ n_vars n2 ++ n_out n2) /\ valid (n_name n2).
+  Proof.
+    intros.
+    induction Hname. induction Hin. induction Hvars. induction Hout.
+    auto.
+  Defined.
+
+  Fact equal_node (n1 n2 : node)
+    (Hname : n_name n1 = n_name n2)
+    (Hstate : n_hasstate n1 = n_hasstate n2)
+    (Hin : n_in n1 = n_in n2)
+    (Hout : n_out n1 = n_out n2)
+    (Hvars : n_vars n1 = n_vars n2)
+    (Heqs : n_eqs n1 = n_eqs n2) :
+    (transport1 Hin (n_ingt0 n1) = n_ingt0 n2) ->
+    (transport2 Hout (n_outgt0 n1) = n_outgt0 n2) ->
+    (transport3 Heqs Hvars Hout (n_defd n1) = n_defd n2) ->
+    (transport4 Hin Hvars Hout Heqs (n_nodup n1) = n_nodup n2) ->
+    (transport5 Hname Hin Hvars Hout (n_good n1) = n_good n2) ->
+    n1 = n2.
+  Proof.
+    intros Heq1 Heq2 Heq3 Heq4 Heq5.
+    destruct n1. destruct n2.
+    simpl in *.
+    destruct Hname. destruct Hstate.
+    destruct Hin. destruct Hout. destruct Hvars.
+    destruct Heqs.
+    simpl in *; subst.
+    reflexivity.
+  Qed.
+
+  Lemma normalized_node_normalize_idem : forall n Hwl,
+      normalized_node n ->
+      normalize_node PS.empty n Hwl = n.
+  Proof with eauto.
+    intros n [G Hwl] Hnormed.
+    unfold normalize_node, normalized_node in *.
+    eapply normalized_equations_normalize_idem
+      with (st:=init_st (first_unused_ident
+                           (self :: out :: map fst (n_in n ++ n_vars n ++ n_out n ++ anon_in_eqs (n_eqs n))))) in Hnormed...
+    destruct n; simpl in *.
+    eapply equal_node; simpl...
+    Unshelve. 6,7,8,9,10:simpl.
+    6,7,8: reflexivity.
+    1,2:reflexivity.
+    4: { rewrite Hnormed; simpl.
+         rewrite init_st_anns; simpl.
+         apply app_nil_r. }
+    4: { rewrite Hnormed... }
+    simpl.
+    1,2,3:apply proof_irrelevance.
+  Qed.
+
+  Corollary normalized_global_normalize_idem : forall G Hwl,
+      normalized_global G ->
+      normalize_global G Hwl = G.
+  Proof with eauto.
+    induction G; intros Hwl Hnormed...
+    simpl. inv Hnormed.
+    eapply normalized_node_normalize_idem in H1...
+    rewrite H1.
+    rewrite IHG...
+  Qed.
+
+  Theorem normalize_global_idem : forall G Hwl1 Hwl2,
+      normalize_global (normalize_global G Hwl1) Hwl2 = normalize_global G Hwl1.
+  Proof.
+    intros G Hwl1 Hwl2.
+    apply normalized_global_normalize_idem.
+    apply normalize_global_normalized_global.
+  Qed.
+End IDEMPOTENCE.
+
+Module IdempotenceFun
+       (Ids : IDS)
+       (Op : OPERATORS)
+       (OpAux : OPERATORS_AUX Op)
+       (Syn : LSYNTAX Ids Op)
+       (Norm : FULLNORM Ids Op OpAux Syn)
+       <: IDEMPOTENCE Ids Op OpAux Syn Norm.
+  Include IDEMPOTENCE Ids Op OpAux Syn Norm.
+End IdempotenceFun.
