src/Lustre/Normalization/LNormalization.v
@@ -2,7 +2,7 @@ From Velus Require Import Common Ident.
 From Velus Require Import Operators Environment.
 From Velus Require Import CoindStreams.
 From Velus Require Import Lustre.LSyntax Lustre.LOrdered Lustre.LTyping Lustre.LClocking Lustre.LSemantics.
-From Velus Require Import Lustre.Normalization.Normalization Lustre.Normalization.Correctness Lustre.Normalization.Completeness.
+From Velus Require Import Lustre.Normalization.FullNorm (* Lustre.Normalization.Correctness *) Lustre.Normalization.Idempotence.
 
 Local Set Warnings "-masking-absolute-name".
 Module Type LNORMALIZATION
@@ -15,9 +15,9 @@ Module Type LNORMALIZATION
        (Import Clo : LCLOCKING Ids Op Syn)
        (Import Lord : LORDERED Ids Op Syn)
        (Import Sem : LSEMANTICS Ids Op OpAux Syn Lord Str).
-  Declare Module Export Norm : NORMALIZATION Ids Op OpAux Syn.
-  Declare Module Export Correct : CORRECTNESS Ids Op OpAux Str Syn Typ Clo Lord Sem Norm.
-  Declare Module Export Complete : COMPLETENESS Ids Op OpAux Syn Typ Norm.
+  Declare Module Norm : FULLNORM Ids Op OpAux Syn.
+  (* Declare Module Export Correct : CORRECTNESS Ids Op OpAux Str Syn Typ Clo Lord Sem Norm. *)
+  Declare Module Idempotence : IDEMPOTENCE Ids Op OpAux Syn Norm.
 End LNORMALIZATION.
 
 Module LNormalizationFun
@@ -31,7 +31,7 @@ Module LNormalizationFun
        (Lord : LORDERED Ids Op Syn)
        (Sem : LSEMANTICS Ids Op OpAux Syn Lord Str)
        <: LNORMALIZATION Ids Op OpAux Str Syn Typ Clo Lord Sem.
-  Module Export Norm := NormalizationFun Ids Op OpAux Syn.
-  Module Export Correct := CorrectnessFun Ids Op OpAux Str Syn Typ Clo Lord Sem Norm.
-  Module Export Complete := CompletenessFun Ids Op OpAux Syn Typ Norm.
+  Module Norm := FullNormFun Ids Op OpAux Syn.
+  (* Module Export Correct := CorrectnessFun Ids Op OpAux Str Syn Typ Clo Lord Sem Norm. *)
+  Module Idempotence := IdempotenceFun Ids Op OpAux Syn Norm.
 End LNormalizationFun.
