src/Lustre/Normalization/Specification.v
@@ -1,0 +1,889 @@
+From Coq Require Import List Sorting.Permutation.
+Import List.ListNotations.
+Open Scope list_scope.
+
+Require Import Omega.
+
+From Velus Require Import Common Ident.
+From Velus Require Import Operators.
+From Velus Require Import Lustre.LSyntax Lustre.LOrdered Lustre.LTyping.
+From Velus Require Import Lustre.Normalization.Fresh Lustre.Normalization.Normalization.
+
+Local Set Warnings "-masking-absolute-name".
+Module Type SPECIFICATION
+       (Import Ids : IDS)
+       (Import Op : OPERATORS)
+       (OpAux : OPERATORS_AUX Op)
+       (Import Syn : LSYNTAX Ids Op)
+       (Import Norm : NORMALIZATION Ids Op OpAux Syn).
+
+  Import Fresh Fresh.Fresh Facts Tactics.
+
+  (** ** Specification of a normalized node *)
+
+  Inductive normalized_lexp : exp -> Prop :=
+  | normalized_Econst : forall c, normalized_lexp (Econst c)
+  | normalized_Evar : forall x ty cl, normalized_lexp (Evar x (ty, cl))
+  | normalized_Eunop : forall op e1 ty cl,
+      normalized_lexp e1 ->
+      normalized_lexp (Eunop op e1 (ty, cl))
+  | normalized_Ebinop : forall op e1 e2 ty cl,
+      normalized_lexp e1 ->
+      normalized_lexp e2 ->
+      normalized_lexp (Ebinop op e1 e2 (ty, cl))
+  | normalized_Ewhen : forall e x b ty cl,
+      normalized_lexp e ->
+      normalized_lexp (Ewhen [e] x b ([ty], cl)).
+
+  Inductive normalized_cexp : exp -> Prop :=
+  | normalized_Emerge : forall x et ef ty cl,
+      normalized_cexp et ->
+      normalized_cexp ef ->
+      normalized_cexp (Emerge x [et] [ef] ([ty], cl))
+  | normalized_Eite : forall e et ef ty cl,
+      normalized_lexp e ->
+      normalized_cexp et ->
+      normalized_cexp ef ->
+      normalized_cexp (Eite e [et] [ef] ([ty], cl))
+  | normalized_lexp_cexp : forall e,
+      normalized_lexp e ->
+      normalized_cexp e.
+
+  Inductive is_constant : exp -> Prop :=
+  | constant_Econst : forall c,
+      is_constant (Econst c)
+  | constant_Ewhen : forall e x b ty cl,
+      is_constant e ->
+      is_constant (Ewhen [e] x b ([ty], cl)).
+
+  Inductive normalized_equation : PS.t -> equation -> Prop :=
+  | normalized_eq_Eapp : forall out xs f es lann,
+      Forall normalized_lexp es ->
+      normalized_equation out (xs, [Eapp f es None lann])
+  | normalized_eq_Eapp_reset : forall out xs f es x ty cl lann,
+      Forall normalized_lexp es ->
+      normalized_equation out (xs, [Eapp f es (Some (Evar x (ty, cl))) lann])
+  | normalized_eq_Efby : forall out x e0 e ann,
+      ~PS.In x out ->
+      is_constant e0 ->
+      normalized_lexp e ->
+      normalized_equation out ([x], [Efby [e0] [e] [ann]])
+  | normalized_eq_cexp : forall out x e,
+      normalized_cexp e ->
+      normalized_equation out ([x], [e]).
+
+  Definition normalized_node (n : node) :=
+    Forall (normalized_equation (ps_from_list (List.map fst (n_out n)))) (n_eqs n).
+
+  Definition normalized_global (G : global) := Forall normalized_node G.
+
+  Hint Constructors is_constant normalized_lexp normalized_cexp normalized_equation.
+
+  (** A few initial properties *)
+
+  Fact constant_normalized_lexp : forall e,
+      is_constant e ->
+      normalized_lexp e.
+  Proof.
+    intros e Hconst.
+    induction Hconst; auto.
+  Qed.
+
+  Fact is_constant_numstreams : forall e,
+      is_constant e ->
+      numstreams e = 1.
+  Proof.
+    intros e Hconst; induction Hconst; reflexivity.
+  Qed.
+
+  Fact normalized_lexp_numstreams : forall e,
+      normalized_lexp e ->
+      numstreams e = 1.
+  Proof.
+    induction e; intros Hnorm; inv Hnorm; reflexivity.
+  Qed.
+
+  Fact normalized_cexp_numstreams : forall e,
+      normalized_cexp e ->
+      numstreams e = 1.
+  Proof.
+    induction e; intros Hnorm; inv Hnorm;
+      try apply normalized_lexp_numstreams in H; auto.
+  Qed.
+
+  (** ** Propagation of the weak_valid_after property *)
+
+  Fact idents_for_anns_weak_valid : forall anns ids st st' out,
+      idents_for_anns anns st = (ids, st') ->
+      weak_valid_after st out ->
+      weak_valid_after st' out.
+  Proof.
+    induction anns; intros ids st st' out Hids Hval;
+      simpl in *; repeat inv_bind; auto.
+    destruct a as [? [? ?]]. repeat inv_bind; eauto.
+  Qed.
+  Local Hint Resolve idents_for_anns_weak_valid.
+
+  Fact idents_for_anns'_weak_valid : forall anns ids st st' out,
+      idents_for_anns' anns st = (ids, st') ->
+      weak_valid_after st out ->
+      weak_valid_after st' out.
+  Proof.
+    induction anns; intros ids st st' out Hids Hval;
+      simpl in *; repeat inv_bind; auto.
+    destruct a as [? [? ?]]. destruct o; repeat inv_bind; [destruct x|]; eauto.
+  Qed.
+  Local Hint Resolve idents_for_anns'_weak_valid.
+
+  Fact init_var_for_clock_weak_valid : forall nck id st st' out,
+      init_var_for_clock nck st = (id, st') ->
+      weak_valid_after st out ->
+      weak_valid_after st' out.
+  Proof.
+    intros nck id st st' out Hinit Hval;
+      unfold init_var_for_clock in Hinit.
+    destruct find in Hinit.
+    - destruct p; inv Hinit; auto.
+    - destruct fresh_ident eqn:Hfresh.
+      inv Hinit; eauto.
+  Qed.
+  Local Hint Resolve init_var_for_clock_weak_valid.
+
+  Fact fby_iteexp_weak_valid : forall e0 e a e' eqs' st st' out,
+      fby_iteexp e0 e a st = (e', eqs', st') ->
+      weak_valid_after st out ->
+      weak_valid_after st' out.
+  Proof.
+    intros e0 e [ty cl] e' eqs' st st' out Hfby Hval;
+      unfold fby_iteexp in Hfby.
+    destruct (Norm.is_constant e0); repeat inv_bind; eauto.
+  Qed.
+  Local Hint Resolve fby_iteexp_weak_valid.
+
+  Fact normalize_fby_weak_valid : forall e0s es anns es' eqs' st st' out,
+      normalize_fby e0s es anns st = (es', eqs', st') ->
+      weak_valid_after st out ->
+      weak_valid_after st' out.
+  Proof.
+    intros e0s es anns es' eqs' st st' out Hfby Hval;
+      unfold normalize_fby in Hfby; repeat inv_bind.
+    eapply map_bind2_weak_valid in H; eauto.
+    eapply Forall_forall; intros [[? ?] [? ?]] Hin ? ? ? ? Hfby Hval'.
+    eapply fby_iteexp_weak_valid in Hval'; eauto.
+  Qed.
+  Local Hint Resolve normalize_fby_weak_valid.
+
+  Fact normalize_reset_weak_valid : forall e e' eqs' st st' out,
+      normalize_reset e st = (e', eqs', st') ->
+      weak_valid_after st out ->
+      weak_valid_after st' out.
+  Proof.
+    intros e e' eqs' st st' out Hnorm Hval.
+    specialize (normalize_reset_spec e) as [[? [? [? Hspec]]]|Hspec]; subst;
+      rewrite Hspec in Hnorm; clear Hspec; repeat inv_bind; auto.
+    destruct hd as [? [? ?]]. repeat inv_bind; eauto.
+  Qed.
+
+  Local Ltac solve_weak_valid :=
+    match goal with
+    | H : map_bind2 _ _ _ = (_, _, ?st) |- weak_valid_after ?st _ =>
+      eapply map_bind2_weak_valid in H; eauto; solve_forall
+    | H : normalize_fby _ _ _ _ = (_, _, ?st) |- weak_valid_after ?st _ =>
+      eapply normalize_fby_weak_valid; eauto
+    | H : normalize_reset _ _ = (_, _, ?st) |- weak_valid_after ?st _ =>
+      eapply normalize_reset_weak_valid; eauto
+    | H : idents_for_anns _ _ = (_, ?st) |- weak_valid_after ?st _ =>
+      eapply idents_for_anns_weak_valid; eauto
+    | H : idents_for_anns' _ _ = (_, ?st) |- weak_valid_after ?st _ =>
+      eapply idents_for_anns'_weak_valid; eauto
+    end.
+
+  Fact normalize_exp_weak_valid : forall e is_control es' eqs' st st' out,
+      normalize_exp is_control e st = (es', eqs', st') ->
+      weak_valid_after st out ->
+      weak_valid_after st' out.
+  Proof with eauto.
+    induction e using exp_ind2; intros is_control es' eqs' st st' out Hnorm Hval;
+      simpl in *; repeat inv_bind...
+    - (* fby *) repeat solve_weak_valid.
+    - (* when *)
+      destruct a; repeat inv_bind. repeat solve_weak_valid.
+    - (* merge *)
+      destruct a; repeat inv_bind.
+      destruct is_control; repeat inv_bind; repeat solve_weak_valid.
+    - (* ite *)
+      destruct a; repeat inv_bind.
+      destruct is_control; repeat inv_bind; repeat solve_weak_valid.
+    - (* app *)
+      destruct ro; repeat inv_bind; repeat solve_weak_valid.
+      eapply H; eauto. repeat solve_weak_valid.
+  Qed.
+  Local Hint Resolve normalize_exp_weak_valid.
+
+  Corollary normalize_exps_weak_valid : forall es es' eqs' st st' out,
+      normalize_exps es st = (es', eqs', st') ->
+      weak_valid_after st out ->
+      weak_valid_after st' out.
+  Proof with eauto.
+    intros es es' eqs' st st' out Hnorm Hval.
+    unfold normalize_exps in Hnorm; repeat inv_bind.
+    eapply map_bind2_weak_valid in H; eauto.
+    eapply Forall_forall; intros ? Hin ? ? ? ? Hnorm Hval'; eauto.
+  Qed.
+  Local Hint Resolve normalize_exps_weak_valid.
+
+  Fact normalize_rhs_weak_valid : forall e keep_fby es' eqs' st st' out,
+      normalize_rhs keep_fby e st = (es', eqs', st') ->
+      weak_valid_after st out ->
+      weak_valid_after st' out.
+  Proof with eauto.
+    destruct e; intros keep_fby es' eqs' st st' out Hnorm Hval;
+      unfold normalize_rhs in Hnorm; eauto.
+    - (* fby *) destruct keep_fby; eauto.
+      repeat inv_bind. repeat solve_weak_valid.
+    - (* app *)
+      destruct o; repeat inv_bind; repeat solve_weak_valid.
+      eapply normalize_exps_weak_valid; eauto.
+  Qed.
+  Hint Resolve normalize_rhs_weak_valid.
+
+  Corollary normalize_rhss_weak_valid : forall es keep_fby es' eqs' st st' out,
+      normalize_rhss keep_fby es st = (es', eqs', st') ->
+      weak_valid_after st out ->
+      weak_valid_after st' out.
+  Proof with eauto.
+    intros es keep_fby es' eqs' st st' out Hnorm Hval.
+    unfold normalize_rhss in Hnorm; repeat inv_bind.
+    eapply map_bind2_weak_valid in H; eauto.
+    eapply Forall_forall; intros ? Hin ? ? ? ? Hnorm Hval'; eauto.
+  Qed.
+  Local Hint Resolve normalize_rhss_weak_valid.
+
+  Fact normalize_equation_weak_valid : forall e to_cut eqs' st st' out,
+      normalize_equation to_cut e st = (eqs', st') ->
+      weak_valid_after st out ->
+      weak_valid_after st' out.
+  Proof with eauto.
+    intros [xs es] to_cut eqs' st st' out Hnorm Hval;
+      unfold normalize_equation in Hnorm; repeat inv_bind; eauto.
+  Qed.
+  Hint Resolve normalize_equation_weak_valid.
+
+  (** ** Additional properties *)
+
+  Fact idents_for_anns_weak_valid_nIn : forall anns ids st st' out,
+      idents_for_anns anns st = (ids, st') ->
+      weak_valid_after st out ->
+      Forall (fun id => ~PS.In id out) (map fst ids).
+  Proof.
+    induction anns; intros ids st st' out Hids Hval;
+      simpl in *; [|destruct a as [? [? ?]]]; repeat inv_bind; simpl; auto.
+    constructor; eauto.
+    eapply fresh_ident_weak_valid_nIn; eauto.
+  Qed.
+
+  (** ** After normalization, equations and expressions are normalized *)
+
+  Fact normalized_lexp_hd_default : forall es,
+      Forall normalized_lexp es ->
+      normalized_lexp (hd_default es).
+  Proof.
+    intros es Hf.
+    destruct es; simpl.
+    - constructor.
+    - inv Hf; auto.
+  Qed.
+
+  Fact map_bind2_normalized_lexp {A A2} :
+    forall (k : A -> FreshAnn ((list exp) * A2)) a es' a2s st st',
+      map_bind2 k a st = (es', a2s, st') ->
+      Forall (fun a => forall es' a2s st st',
+                  k a st = (es', a2s, st') ->
+                  Forall normalized_lexp es') a ->
+      Forall normalized_lexp (concat es').
+  Proof.
+    intros k a eqs' a2s st st' Hmap Hf.
+    apply map_bind2_values in Hmap.
+    induction Hmap; simpl in *.
+    - constructor.
+    - destruct H as [? [? H]]. inv Hf.
+      rewrite Forall_app.
+      split; eauto.
+  Qed.
+
+  Fact map_bind2_normalized_cexp {A A2} :
+    forall (k : A -> FreshAnn ((list exp) * A2)) a es' a2s st st',
+      map_bind2 k a st = (es', a2s, st') ->
+      Forall (fun a => forall es' a2s st st',
+                  k a st = (es', a2s, st') ->
+                  Forall normalized_cexp es') a ->
+      Forall normalized_cexp (concat es').
+  Proof.
+    intros k a eqs' a2s st st' Hmap Hf.
+    apply map_bind2_values in Hmap.
+    induction Hmap; simpl in *.
+    - constructor.
+    - destruct H as [? [? H]]. inv Hf.
+      rewrite Forall_app.
+      split; eauto.
+  Qed.
+
+  Fact add_whens_is_constant : forall ty cl e,
+      is_constant e ->
+      is_constant (add_whens e ty cl).
+  Proof.
+    induction cl; intros e Hcons; simpl.
+    - assumption.
+    - constructor. eauto.
+  Qed.
+
+  Fact add_whens_normalized_lexp : forall ty cl e,
+      normalized_lexp e ->
+      normalized_lexp (add_whens e ty cl).
+  Proof.
+    induction cl; intros e Hadd; simpl in Hadd.
+    - assumption.
+    - constructor. eauto.
+  Qed.
+
+  Hint Resolve in_combine_l in_combine_r.
+  Hint Resolve normalized_lexp_hd_default.
+
+  Fact is_constant_is_constant : forall e,
+      Norm.is_constant e = true <->
+      is_constant e.
+  Proof with eauto.
+    intros e. split; intros Hconst.
+    - induction e using exp_ind2; simpl in Hconst; try congruence.
+      + constructor.
+      + repeat (destruct es; try congruence).
+        inv H; inv H3.
+        destruct a.
+        repeat (destruct l; try congruence).
+        constructor...
+    - induction Hconst...
+  Qed.
+
+  Lemma normalize_exp_normalized_lexp : forall e es' eqs' st st',
+      normalize_exp false e st = (es', eqs', st') ->
+      Forall normalized_lexp es'.
+  Proof with eauto.
+    induction e using exp_ind2; intros es' eqs' st st' Hnorm;
+      simpl in Hnorm; repeat inv_bind; repeat constructor.
+    - (* var *)
+      destruct a...
+    - (* unop *)
+      destruct a...
+    - (* binop *)
+      destruct a. constructor...
+    - (* fby *)
+      repeat rewrite_Forall_forall.
+      repeat simpl_In. destruct a0...
+    - (* when *)
+      destruct a. repeat inv_bind.
+      apply map_bind2_normalized_lexp in H0...
+      repeat rewrite_Forall_forall.
+      repeat simpl_In...
+    - (* merge *)
+      destruct a. repeat inv_bind.
+      repeat rewrite_Forall_forall.
+      repeat simpl_In. destruct a...
+    - (* ite *)
+      destruct a. repeat inv_bind.
+      repeat rewrite_Forall_forall.
+      repeat simpl_In. destruct a...
+    - (* app *)
+      repeat rewrite_Forall_forall.
+      repeat simpl_In. destruct a0...
+  Qed.
+  Hint Resolve normalize_exp_normalized_lexp.
+
+  Corollary normalize_exps_normalized_lexp: forall es es' eqs' st st',
+      normalize_exps es st = (es', eqs', st') ->
+      Forall normalized_lexp es'.
+  Proof.
+    intros es es' eqs' st st' Hnorm.
+    unfold normalize_exps in Hnorm. repeat inv_bind.
+    apply map_bind2_normalized_lexp in H; auto.
+    rewrite Forall_forall; intros; eauto.
+  Qed.
+  Hint Resolve normalize_exps_normalized_lexp.
+
+  Lemma normalize_exp_normalized_cexp : forall e es' eqs' st st',
+      normalize_exp true e st = (es', eqs', st') ->
+      Forall normalized_cexp es'.
+  Proof with eauto.
+    induction e using exp_ind2; intros es' eqs' st st' Hnorm;
+      simpl in Hnorm; repeat inv_bind; repeat constructor.
+    - (* var *)
+      destruct a...
+    - (* unop *)
+      destruct a...
+    - (* binop *)
+      destruct a. constructor...
+    - (* fby *)
+      solve_forall.
+      repeat simpl_In. destruct a0...
+    - (* when *)
+      destruct a. repeat inv_bind.
+      apply map_bind2_normalized_lexp in H0; solve_forall.
+      repeat rewrite_Forall_forall.
+      repeat simpl_In...
+    - (* merge *)
+      destruct a. repeat inv_bind.
+      apply map_bind2_normalized_cexp in H1; solve_forall.
+      apply map_bind2_normalized_cexp in H2; solve_forall.
+      repeat rewrite_Forall_forall.
+      repeat simpl_In...
+    - (* ite *)
+      destruct a. repeat inv_bind.
+      apply normalize_exp_normalized_lexp in H1.
+      apply map_bind2_normalized_cexp in H2; solve_forall.
+      apply map_bind2_normalized_cexp in H3; solve_forall.
+      repeat rewrite_Forall_forall.
+      repeat simpl_In.
+      constructor...
+      apply normalized_lexp_hd_default. solve_forall.
+    - (* app *)
+      solve_forall.
+      repeat simpl_In. destruct a0...
+  Qed.
+
+  Fact init_var_for_clock_normalized_eq : forall cl id eqs' out st st',
+      weak_valid_after st out ->
+      init_var_for_clock cl st = (id, eqs', st') ->
+      Forall (normalized_equation out) eqs'.
+  Proof.
+    intros cl id eqs' out st st' Hvalid Hinit.
+    unfold init_var_for_clock in Hinit.
+    destruct (find _ _).
+    - destruct p. inv Hinit. constructor.
+    - destruct (fresh_ident _ _) eqn:Hfresh. inv Hinit.
+      repeat constructor.
+      + eapply fresh_ident_weak_valid_nIn in Hfresh; eauto.
+      + apply add_whens_is_constant. auto.
+      + apply add_whens_normalized_lexp. auto.
+  Qed.
+
+  Fact fby_iteexp_normalized_eq : forall e0 e a e' eqs' out st st',
+      weak_valid_after st out ->
+      normalized_lexp e ->
+      fby_iteexp e0 e a st = (e', eqs', st') ->
+      Forall (normalized_equation out) eqs'.
+  Proof.
+    intros e0 e [ty cl] e' eqs' out st st' Hvalid He Hfby.
+    unfold fby_iteexp in Hfby.
+    destruct (Norm.is_constant e0); repeat inv_bind; constructor.
+    - assert (weak_valid_after x1 out) as Hvalid' by eauto.
+      constructor; auto.
+      + eapply fresh_ident_weak_valid_nIn in H0; eauto.
+      + eapply add_whens_is_constant; eauto.
+    - eapply init_var_for_clock_normalized_eq in H; eauto.
+  Qed.
+
+  Fact map_bind2_normalized_eq {A A1} :
+    forall (k : A -> FreshAnn (A1 * (list equation))) a out a1s eqs' st st',
+      map_bind2 k a st = (a1s, eqs', st') ->
+      weak_valid_after st out ->
+      (forall a a1s eqs' st st', k a st = (a1s, eqs', st') ->
+                            weak_valid_after st out ->
+                            weak_valid_after st' out) ->
+      Forall (fun a => forall a1s eqs' st st',
+                  k a st = (a1s, eqs', st') ->
+                  weak_valid_after st out ->
+                  Forall (normalized_equation out) eqs') a ->
+      Forall (normalized_equation out) (concat eqs').
+  Proof.
+    induction a; intros out a1s eqs' st st' Hmap Hlt Hfollows Hf;
+      simpl in *; repeat inv_bind.
+    - constructor.
+    - inv Hf. simpl.
+      rewrite Forall_app; eauto.
+  Qed.
+
+  Fact normalize_fby_normalized_eq : forall e0s es anns es' eqs' out st st',
+      weak_valid_after st out ->
+      Forall normalized_lexp es ->
+      normalize_fby e0s es anns st = (es', eqs', st') ->
+      Forall (normalized_equation out) eqs'.
+  Proof with eauto.
+    intros e0s es anns es' eqs' out st st' Hval Hf Hnorm.
+    unfold normalize_fby in Hnorm.
+    repeat inv_bind.
+    - eapply map_bind2_normalized_eq...
+      + intros. destruct a as [[e0 e] [ty cl]]...
+      + rewrite Forall_forall; intros.
+        destruct x as [[e0 e] [ty cl]].
+        eapply fby_iteexp_normalized_eq in H1...
+        rewrite Forall_forall in Hf...
+  Qed.
+
+  Lemma normalize_exp_normalized_eq : forall e is_control es' eqs' out st st',
+      weak_valid_after st out ->
+      normalize_exp is_control e st = (es', eqs', st') ->
+      Forall (normalized_equation out) eqs'.
+  Proof with eauto.
+    induction e using exp_ind2; intros is_control es' eqs' out st st' Hval Hnorm;
+      simpl in Hnorm; repeat inv_bind; repeat constructor; eauto.
+    - (* binop *)
+      apply Forall_app. split...
+    - (* fby *)
+      assert (weak_valid_after x1 out) as Hvalid1 by solve_weak_valid.
+      assert (weak_valid_after x4 out) as Hvalid2 by solve_weak_valid.
+      assert (weak_valid_after x7 out) as Hvalid3 by solve_weak_valid.
+      repeat rewrite Forall_app. repeat split.
+      + apply map_bind2_normalized_lexp in H1; [| solve_forall].
+        apply map_bind2_normalized_lexp in H2; [| solve_forall].
+        clear H H0.
+        unfold normalize_fby in H3; repeat inv_bind. apply map_bind2_values in H.
+        repeat rewrite_Forall_forall.
+        repeat simpl_In.
+        apply In_nth with (d:=(hd_default [])) in H6; destruct H6 as [n [? ?]].
+        replace (length x5) in H6.
+        specialize (H3 (e, e, a0) (hd_default []) [] _ _ _ _ H6 eq_refl eq_refl eq_refl). destruct H3 as [? [? H3]].
+        destruct (nth n _) as [[e0 e'] [ty cl]] eqn:Hnth.
+        unfold fby_iteexp in H3.
+        destruct (Norm.is_constant e0) eqn:Hisconst; repeat inv_bind.
+        * simpl in *. rewrite <- H9. repeat constructor.
+          -- intro contra.
+             eapply idents_for_anns_weak_valid_nIn in H4...
+             rewrite Forall_forall in H4. apply H4 in contra; auto.
+             rewrite in_map_iff. exists (i, a0); auto.
+          -- rewrite is_constant_is_constant in Hisconst...
+          -- eapply nth_In in H6; rewrite Hnth in H6...
+        * simpl. rewrite <- H11. repeat constructor.
+          eapply nth_In in H6; rewrite Hnth in H6...
+      + eapply map_bind2_normalized_eq in H1... solve_forall.
+      + eapply map_bind2_normalized_eq in H2...
+        * eapply map_bind2_st_follows in H1; solve_forall.
+      + eapply normalize_fby_normalized_eq in H3; eauto.
+        eapply map_bind2_normalized_lexp; eauto. solve_forall.
+    - (* when *)
+      destruct a. repeat inv_bind.
+      eapply map_bind2_normalized_eq in H0; eauto. solve_forall.
+    - (* merge *)
+      destruct a; destruct is_control; repeat inv_bind;
+        repeat rewrite Forall_app; repeat split.
+      1,2,4,5: (eapply map_bind2_normalized_eq; eauto; solve_forall).
+      1,2: solve_weak_valid.
+      rewrite Forall_forall; intros [? ?] Hin. rewrite map_map in Hin; simpl in Hin.
+      repeat simpl_In.
+      constructor. constructor.
+      + eapply map_bind2_normalized_cexp in H1; eauto; solve_forall.
+        rewrite Forall_forall in H1...
+        eapply normalize_exp_normalized_cexp...
+      + eapply map_bind2_normalized_cexp in H2; eauto; solve_forall.
+        rewrite Forall_forall in H2...
+        eapply normalize_exp_normalized_cexp...
+    - (* ite *)
+      destruct a; destruct is_control; repeat inv_bind;
+        repeat rewrite Forall_app; repeat split.
+      1,5: (eapply IHe; eauto).
+      1,2,4,5: (eapply map_bind2_normalized_eq; eauto; solve_forall).
+      1,2: solve_weak_valid.
+      rewrite Forall_forall; intros [? ?] Hin. rewrite map_map in Hin; simpl in Hin.
+      repeat simpl_In.
+      constructor. constructor.
+      + eapply normalized_lexp_hd_default.
+        eapply normalize_exp_normalized_lexp...
+      + eapply map_bind2_normalized_cexp in H2; eauto; solve_forall.
+        rewrite Forall_forall in H2...
+        eapply normalize_exp_normalized_cexp...
+      + eapply map_bind2_normalized_cexp in H3; eauto; solve_forall.
+        rewrite Forall_forall in H3...
+        eapply normalize_exp_normalized_cexp...
+    - (* app *)
+      eapply map_bind2_normalized_lexp in H1; eauto; solve_forall.
+      destruct ro; repeat inv_bind.
+      + specialize (normalize_reset_spec (hd_default x)) as [[? [? [? Hspec]]]|Hspec]; subst;
+          rewrite Hspec in H4; clear Hspec; repeat inv_bind.
+        * destruct x3...
+        * destruct (hd _) as [? [? ?]]; simpl in *; repeat inv_bind...
+      + constructor...
+    - (* app (auxiliary equations) *)
+      rewrite Forall_app. split.
+      + destruct ro; repeat inv_bind;
+        eapply map_bind2_normalized_eq in H1; eauto; solve_forall.
+      + destruct ro; repeat inv_bind; try constructor;
+        eapply Forall_app. split.
+        * eapply H in H2... solve_weak_valid.
+        * specialize (normalize_reset_spec (hd_default x)) as [[? [? [? Hspec]]]|Hspec]; subst;
+          rewrite Hspec in H4; clear Hspec; repeat inv_bind...
+          destruct (hd _) as [? [? ?]]; simpl in *; repeat inv_bind.
+          repeat constructor. apply normalized_lexp_hd_default...
+  Qed.
+  Local Hint Resolve normalize_exp_normalized_eq.
+
+  Corollary normalize_exps_normalized_eq : forall es es' eqs' out st st',
+      weak_valid_after st out ->
+      normalize_exps es st = (es', eqs', st') ->
+      Forall (normalized_equation out) eqs'.
+  Proof.
+    intros es es' eqs' out st st' Hval Hnorm.
+    unfold normalize_exps in Hnorm. repeat inv_bind.
+    eapply map_bind2_normalized_eq in H; eauto.
+    solve_forall.
+  Qed.
+  Local Hint Resolve normalize_exps_normalized_eq.
+
+  (* Intermediary predicate for normalized rhs *)
+  Inductive normalized_rhs : bool -> exp -> Prop :=
+  | normalized_rhs_Eapp : forall f es lann keep_fby,
+      Forall normalized_lexp es ->
+      normalized_rhs keep_fby (Eapp f es None lann)
+  | normalized_rhs_Eapp_reset : forall f es x ty cl lann keep_fby,
+      Forall normalized_lexp es ->
+      normalized_rhs keep_fby (Eapp f es (Some (Evar x (ty, cl))) lann)
+  | normalized_rhs_Efby : forall e0 e ann,
+      is_constant e0 ->
+      normalized_lexp e ->
+      normalized_rhs true (Efby [e0] [e] [ann])
+  | normalized_rhs_cexp : forall e keep_fby,
+      normalized_cexp e ->
+      normalized_rhs keep_fby e.
+  Hint Constructors normalized_rhs.
+
+  Fact normalized_equation_normalized_rhs : forall xs es to_cut,
+      normalized_equation to_cut (xs, es) ->
+      Forall (normalized_rhs (negb (existsb (fun x => PS.mem x to_cut) xs))) es.
+  Proof with eauto.
+    intros xs es to_cut Hnormed.
+    inv Hnormed...
+    constructor; [| constructor].
+    simpl.
+    apply PSE.mem_3 in H1. rewrite H1; simpl...
+  Qed.
+
+  Fact normalize_rhs_normalized_rhs : forall e keep_fby es' eqs' st st',
+      normalize_rhs keep_fby e st = (es', eqs', st') ->
+      Forall (normalized_rhs keep_fby) es'.
+  Proof with eauto.
+    intros e keep_fby es' eqs' st st' Hnorm.
+    destruct e; unfold normalize_rhs in Hnorm;
+      try (apply normalize_exp_normalized_cexp in Hnorm; solve_forall; auto).
+    - (* fby *)
+      destruct keep_fby; try (apply normalize_exp_normalized_cexp in Hnorm; solve_forall; auto).
+      repeat inv_bind.
+      apply normalize_exps_normalized_lexp in H.
+      apply normalize_exps_normalized_lexp in H0.
+      unfold normalize_fby in H1. repeat inv_bind.
+      apply map_bind2_values in H1.
+      repeat rewrite_Forall_forall.
+      apply In_nth with (d:=(hd_default [])) in H4; destruct H4 as [n [Hn Hnth]].
+      replace (length es') in Hn.
+      specialize (H3 (x5, x5, (bool_type, (Cbase, None))) (hd_default []) [] _ _ _ _ Hn eq_refl eq_refl eq_refl).
+      destruct H3 as [? [? H3]]. destruct (nth n _ _) as [[e0 e] [ty cl]] eqn:Hnth'.
+      unfold fby_iteexp in H3.
+      destruct (Norm.is_constant e0) eqn:Hisconst; repeat inv_bind; simpl in *.
+      + rewrite <- H5. repeat constructor.
+        * rewrite is_constant_is_constant in Hisconst...
+        * eapply nth_In in Hn. rewrite Hnth' in Hn...
+      + rewrite <- H7. repeat constructor.
+        eapply nth_In in Hn. rewrite Hnth' in Hn...
+    - (* app *)
+      destruct o; repeat inv_bind...
+      specialize (normalize_reset_spec (hd_default x4)) as [[? [[? ?] [? Hspec]]]|Hspec]; subst;
+        rewrite Hspec in H1; clear Hspec; repeat inv_bind...
+      destruct (hd _) as [? [ty cl]]; simpl in H1. repeat inv_bind...
+  Qed.
+
+  Corollary normalize_rhss_normalized_rhs : forall es keep_fby es' eqs' st st',
+      normalize_rhss keep_fby es st = (es', eqs', st') ->
+      Forall (normalized_rhs keep_fby) es'.
+  Proof with eauto.
+    intros es keep_fby es' eqs' st st' Hnorm.
+    unfold normalize_rhss in Hnorm. repeat inv_bind.
+    eapply map_bind2_values in H.
+    induction H; simpl; try constructor.
+    apply Forall_app. split; auto.
+    destruct H as [? [? H]].
+    eapply normalize_rhs_normalized_rhs; eauto.
+  Qed.
+
+  Fact normalize_rhs_normalized_eq : forall e keep_fby es' eqs' out st st',
+      weak_valid_after st out ->
+      normalize_rhs keep_fby e st = (es', eqs', st') ->
+      Forall (normalized_equation out) eqs'.
+  Proof with eauto.
+    intros e keep_fby es' eqs' out st st' Hval Hnorm.
+    destruct e; unfold normalize_rhs in Hnorm;
+      try (eapply normalize_exp_normalized_eq in Hnorm; eauto).
+    - (* fby *)
+      destruct keep_fby; try (eapply normalize_exp_normalized_eq in Hnorm; eauto).
+      simpl in Hnorm. repeat inv_bind.
+      repeat rewrite Forall_app. repeat split...
+      + eapply normalize_fby_normalized_eq in H1; eauto.
+    - (* app *)
+      repeat inv_bind...
+      destruct o; repeat inv_bind; repeat rewrite Forall_app; repeat split...
+      specialize (normalize_reset_spec (hd_default x4)) as [[? [? [? Hspec]]]|Hspec]; subst;
+        rewrite Hspec in H1; clear Hspec; repeat inv_bind; eauto.
+      + destruct (hd _ _) as [? [? ?]]; simpl in H1.
+        repeat inv_bind. repeat constructor.
+        apply normalized_lexp_hd_default...
+  Qed.
+  Hint Resolve normalize_rhs_normalized_eq.
+
+  Corollary normalize_rhss_normalized_eq : forall es keep_fby es' eqs' out st st',
+      weak_valid_after st out ->
+      normalize_rhss keep_fby es st = (es', eqs', st') ->
+      Forall (normalized_equation out) eqs'.
+  Proof.
+    intros es keep_fby es' eqs' out st st' Hvalid Hnorm.
+    unfold normalize_rhss in Hnorm; repeat inv_bind.
+    eapply map_bind2_normalized_eq in H; eauto.
+    rewrite Forall_forall; intros; eauto.
+  Qed.
+  Hint Resolve normalize_rhss_normalized_eq.
+
+  Lemma normalize_equation_normalized_eq : forall G eq to_cut eqs' out st st',
+      weak_valid_after st out ->
+      wl_equation G eq ->
+      normalize_equation to_cut eq st = (eqs', st') ->
+      PS.Subset out to_cut ->
+      Forall (normalized_equation out) eqs'.
+  Proof with eauto.
+    intros G [xs es] to_cut eqs' out st st' Hval Hwl Hnorm Hincl.
+    unfold normalize_equation in Hnorm.
+    repeat inv_bind.
+    remember (negb (existsb (fun x => PS.mem x to_cut) xs)) as keep_fby.
+    assert (keep_fby = true -> Forall (fun x => ~PS.In x out) xs) as Hin.
+    { intro Hkeep; subst.
+      rewrite Bool.negb_true_iff in Hkeep. rewrite existsb_Forall in Hkeep.
+      rewrite forallb_Forall in Hkeep. solve_forall.
+      rewrite Bool.negb_true_iff in H0. apply PSE.mem_4 in H0.
+      intro contra. apply Hincl in contra. contradiction.
+    }
+    clear Heqkeep_fby.
+    rewrite Forall_app. split.
+    - assert (length xs = length (annots x)) as Hlen.
+      { destruct Hwl as [Hwl1 Hwl2].
+        eapply normalize_rhss_annots in H; eauto.
+        congruence. } clear Hwl.
+      eapply normalize_rhss_normalized_rhs in H; eauto.
+      revert xs Hin Hlen.
+      induction H; intros xs Hin Hlen; constructor.
+      + inv H...
+        * destruct xs; simpl in *; try omega.
+          constructor...
+          specialize (Hin eq_refl). inv Hin. auto.
+        * simpl in Hlen. rewrite app_length in Hlen.
+          rewrite length_annot_numstreams in Hlen.
+          specialize (normalized_cexp_numstreams _ H1) as Hlen'.
+          rewrite Hlen' in *. simpl.
+          destruct xs... simpl in Hlen. omega.
+      + eapply IHForall.
+        * intro Hkeep. apply Hin in Hkeep.
+          apply Forall_skipn...
+        * rewrite skipn_length.
+          rewrite Hlen. simpl. rewrite app_length.
+          rewrite length_annot_numstreams. omega.
+    - eapply normalize_rhss_normalized_eq in H; eauto.
+  Qed.
+
+  Corollary normalize_equations_normalized_eq : forall G eqs to_cut eqs' out st st',
+      weak_valid_after st out ->
+      Forall (wl_equation G) eqs ->
+      normalize_equations to_cut eqs st = (eqs', st') ->
+      PS.Subset out to_cut ->
+      Forall (normalized_equation out) eqs'.
+  Proof.
+    induction eqs; intros to_cut eqs' out st st' Hval Hwl Hnorm Hincl;
+      simpl in Hnorm; repeat inv_bind; auto.
+    inv Hwl. apply Forall_app; split.
+    - eapply normalize_equation_normalized_eq; eauto.
+    - eapply IHeqs in H0; eauto.
+  Qed.
+
+  (** ** No anonymous names in a normalized node *)
+
+  Fact is_constant_no_fresh : forall e,
+      is_constant e ->
+      fresh_in e = [].
+  Proof with eauto.
+    intros e Hconst.
+    induction Hconst; simpl...
+    rewrite IHHconst...
+  Qed.
+
+  Fact normalized_lexp_no_fresh : forall e,
+      normalized_lexp e ->
+      fresh_in e = [].
+  Proof with eauto.
+    intros e Hnormed.
+    induction Hnormed; simpl...
+    - (* binop *)
+      rewrite IHHnormed1. rewrite IHHnormed2. reflexivity.
+    - (* when *)
+      rewrite IHHnormed. reflexivity.
+  Qed.
+
+  Fact normalized_cexp_no_fresh : forall e,
+      normalized_cexp e ->
+      fresh_in e = [].
+  Proof with eauto.
+    intros e Hnormed.
+    induction Hnormed; simpl...
+    - (* merge *)
+      rewrite IHHnormed1. rewrite IHHnormed2. reflexivity.
+    - (* ite *)
+      rewrite IHHnormed1. rewrite IHHnormed2.
+      rewrite normalized_lexp_no_fresh...
+    - (* lexp *)
+      eapply normalized_lexp_no_fresh...
+  Qed.
+
+  Fact normalized_equation_no_anon_in_eq : forall to_cut e,
+      normalized_equation to_cut e ->
+      anon_in_eq e = [].
+  Proof with eauto.
+    intros to_cut e Hnormed.
+    induction Hnormed; unfold anon_in_eq, anon_ins; simpl; repeat rewrite app_nil_r.
+    - (* app *)
+      unfold fresh_ins. rewrite concat_eq_nil, Forall_map.
+      solve_forall. eapply normalized_lexp_no_fresh...
+    - (* app (reset) *)
+      unfold fresh_ins. rewrite concat_eq_nil, Forall_map.
+      solve_forall. eapply normalized_lexp_no_fresh...
+    - (* fby *)
+      rewrite is_constant_no_fresh...
+      rewrite normalized_lexp_no_fresh...
+    - (* cexp *)
+      specialize (anon_in_fresh_in e) as Hincl.
+      rewrite normalized_cexp_no_fresh in Hincl...
+      apply incl_nil...
+  Qed.
+
+  Lemma normalized_equations_no_anon : forall to_cut eqs,
+      Forall (normalized_equation to_cut) eqs ->
+      anon_in_eqs eqs = [].
+  Proof.
+    intros to_cut eqs Hnormed.
+    unfold anon_in_eqs.
+    rewrite concat_eq_nil, Forall_map.
+    solve_forall. eapply normalized_equation_no_anon_in_eq; eauto.
+  Qed.
+
+  Corollary normalize_equations_no_anon : forall G eqs to_cut eqs' out st st',
+      weak_valid_after st out ->
+      Forall (wl_equation G) eqs ->
+      normalize_equations to_cut eqs st = (eqs', st') ->
+      PS.Subset out to_cut ->
+      anon_in_eqs eqs' = [].
+  Proof.
+    intros G eqs to_cut eqs' out st st' Hval Hwl Hnorm Hsub.
+    eapply normalized_equations_no_anon.
+    eapply normalize_equations_normalized_eq; eauto.
+  Qed.
+
+End SPECIFICATION.
+
+Module SpecificationFun
+       (Ids : IDS)
+       (Op : OPERATORS)
+       (OpAux : OPERATORS_AUX Op)
+       (Syn : LSYNTAX Ids Op)
+       (Norm : NORMALIZATION Ids Op OpAux Syn)
+       <: SPECIFICATION Ids Op OpAux Syn Norm.
+  Include SPECIFICATION Ids Op OpAux Syn Norm.
+End SpecificationFun.
